Some refactoring on tm_floatarith.

Experiments.thy
@@ -3,7 +3,7 @@ imports Taylor_Models
 begin
 
 (* Trying out arithmetic on intervals and polynomials with interval coefficients. *)
-(*value "Ivl (-1::float) 1 + Ivl 0 1"
+value "Ivl (-1::float) 1 + Ivl 0 1"
 value "Ivl (-8::float) 2 + Ivl (-2) (-1)"
 value "Ivl (0::real) 1 * Ivl 0 1"
 value "Ivl (-10::real) 6 * Ivl (-4) 2"
@@ -15,7 +15,7 @@ value "compute_bound_fa 64 (Add (Var 0) (Num 3)) [Ivl 1 2]"
 
 value "map_option (interval_map real_of_float) (compute_bound_fa 16 (Cos (Var 0)) [Ivl (-1) 1])"
 
-value "map (interval_map real_of_float) (the (tmf_cs 32 10 (Ivl 0 2) 1 (Cos (Var 0))))"
+value "map (interval_map real_of_float) (the (tmf_ivl_poly 32 10 (Ivl 0 2) 1 (Cos (Var 0))))"
 
 (* Compute some taylor models. *)
 value "the (compute_tm 32 7 [Ivl 0 2] [1] (Num 2))"
@@ -24,21 +24,28 @@ value "the (compute_tm 32 7 [Ivl 0 2, Ivl 0 2] [1,1] (Add (Var 0) (Var 1)))"
 value "tm_norm_poly (the (compute_tm 32 10 [Ivl (-1) 1] [0] (Cos (Var 0))))"
 value [code] "tm_norm_poly (the (compute_tm 32 7 [Ivl (-1) 1, Ivl (-1) 1] [0, 0] (Add (Exp (Add (Var 0) (Var 1))) (Cos (Mult (Var 0) (Var 1))))))"
 
-value "let I = [Ivl 1 3]; a = [2] in case (the (compute_tm 32 10 I a (Inverse (Var 0)))) of TaylorModel p e \<Rightarrow> (tm_lower_order 5 (TaylorModel p e) I a)"
+value "real_of_rat (Fract 10 3) "
 
-value "map_option (interval_map real_of_float) (compute_ivl_bound 32 10 [Ivl (-1) 1] (Power (Cos (Var 0)) 2))"
-value "map_option (interval_map real_of_float) (compute_ivl_bound 32 10 [Ivl (1) 2] (Inverse (Add (Cos (Var 0)) (Num 2))))"
-value "map_option (interval_map real_of_float) (compute_ivl_bound 32 10 [Ivl (1) 2] (Inverse (Var 0)))"*)
 
-(*definition "test (u::unit) = prove_pos 50 40 (FloatR 1 (-3)) (FloatR 1 (-1)) caprasse (aform_of_ivl (mk_tuple4 (- FloatR 1 (-1))) (mk_tuple4 (FloatR 1 (-1))))"*)
-definition "test (u::unit) = the (compute_tm 32 7 [Ivl 0 2, Ivl 0 2] [1,1] (Add (Var 0) (Var 1)))"
+(* Some performance tests. *)
+definition "test_expr = (Add (Power (Cos (Var 0)) 2) (Power (Sin (Var 0)) 2))"
 
-ML \<open>val test = @{code test}\<close>
+definition "n = 5"
+definition "prec = 32"
 
-ML \<open>test ()\<close>
-ML \<open>Timing.timeit test\<close>
+definition "test_naive (u::unit) = compute_ivl_bound_naive prec n test_expr [Ivl 0 10]"
+definition "test_best (u::unit) = compute_ivl_bound_subdiv prec 5 n test_expr [Ivl 0 10]"
 
-definition "approx_cos I = (case the (compute_tm 32 10 I (map mid I) (Cos (Var 0))) of TaylorModel p e \<Rightarrow> (p, e))"
+ML \<open>val test_best = @{code test_best}\<close>
+ML \<open>val test_naive = @{code test_best}\<close>
+
+value "test_best ()"
+value "test_naive ()"
+
+ML \<open>Timing.timeit test_best\<close>
+ML \<open>Timing.timeit test_naive\<close>
+
+(*definition "approx_cos I = (case the (compute_tm 32 10 I (map mid I) (Cos (Var 0))) of TaylorModel p e \<Rightarrow> (p, e))"
 
 fun approx_cos_error
 where "approx_cos_error I = snd (approx_cos [Ivl (-1) 1])"
@@ -66,6 +73,19 @@ value "approx_cos_naive [Ivl 5 7]"
 value "approx_cos_naive [Ivl 7 9]"
 value "approx_cos_naive [Ivl 9 11]"
 
+(*
+Direct evaluation of the approximation polynomial:
+cos(09.00): -0.9111303674289957
+cos(09.25): -0.9847651789784349
+cos(09.50): -0.9971721560252718
+cos(09.75): -0.9475798037387368
+cos(10.00): -0.8390715288696811
+cos(10.25): -0.6783938503053173
+cos(10.50): -0.4755369279566821
+cos(10.75): -0.24311342716018713
+cos(11.00):  0.00442561914678663
+*)
+
 value "approx_cos_trans [Ivl (-1) 1]"
 value "approx_cos_trans [Ivl 1 3]"
 value "approx_cos_trans [Ivl 3 5]"
@@ -85,7 +105,7 @@ value "approx_cos_naive [Ivl (-11) (-9)]"
 value "approx_cos_trans [Ivl (-11) (-9)]"
 value "approx_cos_best [Ivl (-11) (-9)]"
 
-(*value "the (compute_tm 32 10 [Ivl (-1) 1] [0] (Cos (Var 0)))"
+value "the (compute_tm 32 10 [Ivl (-1) 1] [0] (Cos (Var 0)))"
 value "the (compute_tm 32 10 [Ivl (-1) 1] [0] (Cos (Add (Var 0) (Mult (Num 2) Pi))))"
 value "the (compute_tm 32 10 [Ivl 9 11] [10] (Cos (Var 0)))"
 value "the (compute_tm 32 10 [Ivl (-10) 10] [0] (Cos (Var 0)))"
